\documentclass[12pt]{article}
\usepackage{amsmath, amssymb, graphicx}
\usepackage{geometry}
\geometry{a4paper, margin=1in}

\begin{document}

\begin{center}
    {\LARGE\textbf{CSE 547: Assignment Number 1}} \\[1em]
    {\large Amirhossein Najafizadeh} \\[1em]
    Semester: Fall 2024 \\ 
    University Number: 116715544 \\[1em]
    \noindent\rule{\textwidth}{0.6pt}
\end{center}

\section{Example Problems}
\subsection{Problem 1}
\textbf{Statement:} Prove that the sum of the first $n$ natural numbers is given by:
\[
S = \frac{n(n+1)}{2}
\]

\textbf{Solution:} We can prove this using mathematical induction.

\textit{Base Case:} For $n = 1$, the sum $S = 1$, which matches the formula.

\textit{Inductive Step:} Assume the formula is true for $n = k$, i.e.,
\[
S = \frac{k(k+1)}{2}
\]
Now, consider $n = k+1$. The sum for $n = k+1$ is:
\[
S = \frac{k(k+1)}{2} + (k+1) = \frac{k(k+1) + 2(k+1)}{2} = \frac{(k+1)(k+2)}{2}
\]
Thus, the formula holds for $n = k+1$. By induction, the formula is true for all $n \in \mathbb{N}$.

% Exercises
\section{Exercises}
\subsection{Exercise 1}
Prove that the binomial coefficient $\binom{n}{k}$ satisfies the identity:
\[
\binom{n}{k} = \binom{n-1}{k} + \binom{n-1}{k-1}
\]

\subsection{Exercise 2}
Evaluate the following sum:
\[
\sum_{k=1}^{n} k^2
\]

\end{document}
